Add new semantics tests, including wal test
This commit also updates the generated test files to initialize a disk
of size 30 for each test. The corresponding commit in perennial does the
same.

cmd/test_gen/main.go
@@ -27,6 +27,7 @@ package semantics
 
 import (
 	"github.com/stretchr/testify/suite"
+	"github.com/tchajed/goose/machine/disk"
 	"testing"
 )
 
@@ -159,6 +160,8 @@ func main() {
 
 				if len(m) != 0 {
 					fmt.Fprintf(out, "func (suite *GoTestSuite) Test%s() {\n", m[3])
+					fmt.Fprintf(out, "\td := disk.NewMemDisk(30)\n")
+					fmt.Fprintf(out, "\tdisk.Init(d)\n")
 					fmt.Fprintf(out, "\tsuite.Equal(true, %stest%s())\n", m[2], m[3])
 					fmt.Fprintf(out, "}\n\n")
 				}
